src/program_proof/mvcc/txn_do_txn.v
@@ -3,27 +3,25 @@ From Perennial.program_proof.mvcc Require Import mvcc_inv txn_common txn_begin t
 Section program.
 Context `{!heapGS Σ, !mvcc_ghostG Σ}.
 
-Definition txnmap_ptstos τ (m : dbmap) : iProp Σ :=
-  [∗ map] k ↦ v ∈ m, txnmap_ptsto τ k v.
-
-Definition dbmap_ptstos γ (m : dbmap) : iProp Σ :=
-  [∗ map] k ↦ v ∈ m, dbmap_ptsto γ k v.
-
-Definition spec_body (body : val) (txn :loc) r P Q τ : iProp Σ :=
-  {{{ ⌜P r⌝ ∗ txnmap_ptstos τ r }}}
+Definition spec_body (body : val) (txn :loc) r P Q γ τ : iProp Σ :=
+  {{{ own_txn txn γ τ ∗ ⌜P r⌝ ∗ txnmap_ptstos τ r }}}
     body #txn
-  {{{ w (ok : bool), RET #ok; if ok then ⌜Q r w⌝ ∗ txnmap_ptstos τ w else True }}}.
+  {{{ w (ok : bool), RET #ok;
+      own_txn txn γ τ ∗
+      if ok then ⌜Q r w⌝ ∗ txnmap_ptstos τ w else True
+  }}}.
 
 Theorem wp_txn__DoTxn txn (body : val) P Q γ :
   (∀ r w, (Decision (Q r w))) ->
-  ⊢ {{{ own_txn_uninit txn γ ∗ (∀ r τ, spec_body body txn r P Q τ) }}}
+  ⊢ {{{ own_txn_uninit txn γ ∗ (∀ r τ, spec_body body txn r P Q γ τ) }}}
     <<< ∀∀ (r : dbmap), ⌜P r⌝ ∗ dbmap_ptstos γ r >>>
       Txn__DoTxn #txn body @ ↑mvccNSST
     <<< ∃∃ (ok : bool), if ok then (∃ w, ⌜Q r w⌝ ∗ dbmap_ptstos γ w) else dbmap_ptstos γ r >>>
+    (* We put [v] here as a placeholder; also, there seems to be no notation for no-binder case. *)
     {{{ (v : u64), RET #ok; own_txn_uninit txn γ }}}.
 Proof.
   iIntros (Hdec) "!>".
-  iIntros (Φ) "[Htxn Hbody] HAU".
+  iIntros (Φ) "[Htxn #Hbody] HAU".
   wp_call.
 
   (***********************************************************)
@@ -36,18 +34,58 @@ Proof.
   (* txn.Commit()                                            *)
   (* return true                                             *)
   (***********************************************************)
+  iAssert (∃ p, mvcc_inv_sst γ p)%I with "[Htxn]" as (p) "#Hinv".
+  { iNamed "Htxn". eauto with iFrame. }
   wp_apply (wp_txn__Begin with "Htxn").
-  iIntros "[%τ Htxn]".
-  wp_pures.
-  wp_apply ("Hbody").
-  { (* TODO: Prove precondition. *) admit. }
-  iIntros (w ok) "H".
-  wp_pures.
-  wp_if_destruct.
-  { (* Abort branch. *) admit. }
-  wp_apply (wp_txn__Commit with "Htxn").
-  iIntros (ok) "Htxn".
-  wp_pures.
+  iInv "Hinv" as "> HinvO" "HinvC".
+  replace (⊤ ∖ ∅) with (⊤ : coPset) by set_solver.
+  iMod "HAU" as (r) "[[%HP Hdbps] HAUC]".
+  iModIntro.
+  iNamed "HinvO".
+  iExists ts.
+  iFrame "Hts".
+  iIntros "(%n & Hts & %Hn)".
+  (* Obtain [ltuple_ptsto] over [m]. *)
+  iMod (per_key_inv_ltuple_ptstos with "Hkeys") as "[Hkeys Hltuples]".
+  iDestruct (dbmap_lookup_big with "Hm Hdbps") as "%Hrm". 
+  (* Obtain [ltuple_ptsto] over [r]. *)
+  iDestruct (big_sepM_subseteq _ _ r with "Hltuples") as "Hltuples"; first auto.
+  (* Obtain [txnmap_auth] and [txnmap_ptsto]. *)
+  iMod (txnmap_alloc r) as (τ) "[Htxnmap Htxnps]".
+  pose proof (spec_peek future (U64 ts)).
+  destruct (peek future (U64 ts)).
+  { (* Case NCA. *)
+    iMod ("HAUC" $! false with "Hdbps") as "HΦ".
+    (* TODO: Add [tid] to [tmods_nca] and get a piece of evidence. *)
+    iMod ("HinvC" with "[- HΦ Hltuples Htxnmap Htxnps ]") as "_".
+    { (* TODO: close the inv. *) admit. }
+    iIntros "!>" (tid) "[Htxn %Etid]".
+    iAssert (own_txn txn γ τ)%I with "[Hltuples Htxnmap Htxn]" as "Htxn".
+    { iExists _, r, ∅. rewrite map_empty_union. iFrame. }
+    wp_pures.
+    wp_apply ("Hbody" with "[$Htxn $Htxnps]"); first auto.
+    iIntros (w ok) "[Htxn Hpost]".
+    wp_pures.
+    wp_if_destruct.
+    { (* Abort branch. *) admit. }
+    wp_apply (wp_txn__Commit with "Htxn").
+    iIntros (ok) "Htxn".
+    wp_pures.
+    admit.
+  }
+  { (* Case FA. *)
+    admit.
+  }
+  { (* Case FCI. *)
+    admit.
+  }
+  destruct (decide (Q r (mods ∪ r))); last first.
+  { (* Case FCC, [Q r (w ∪ m)] not holds. *)
+    admit.
+  }
+  { (* Case FCC, [Q r (w ∪ m)] holds. *)
+    admit.
+  }
 Admitted.
 
 
@@ -56,10 +94,13 @@ Admitted.
 Definition post_Swap (r w : dbmap) : Prop.
 Admitted.
 
-Theorem wp_SwapSeq txn r τ :
-  {{{ ⌜pre_Swap r⌝ ∗ txnmap_ptstos τ r }}}
+Theorem wp_SwapSeq txn r γ τ :
+  {{{ own_txn txn γ τ ∗ ⌜pre_Swap r⌝ ∗ txnmap_ptstos τ r }}}
     SwapSeq #txn
-  {{{ w (ok : bool), RET #ok; if ok then ⌜post_Swap r w⌝ ∗ txnmap_ptstos τ w else True }}}.
+  {{{ w (ok : bool), RET #ok;
+      own_txn txn γ τ ∗
+      if ok then ⌜post_Swap r w⌝ ∗ txnmap_ptstos τ w else True
+  }}}.
 Admitted.
 
 Instance post_Swap_dec : (∀ r w, (Decision (post_Swap r w))).
