src/program_proof/mvcc/tuple_read_version.v
@@ -194,18 +194,18 @@ Definition tuple_read tuple tid key val found γ : iProp Σ :=
     "%Htid" ∷ ⌜int.Z tid ≤ int.Z tidlast ∨ int.Z tidown = 0⌝ ∗
     "%Hret" ∷ ⌜spec_lookup vers tid = to_dbval found val⌝.
 
-Definition per_key_cmt_inv_def key tmods m past future γ : iProp Σ :=
-  per_key_inv_def γ key tmods m past ∗ cmt_inv_def γ tmods future.
+Definition per_key_cmt_inv_def key tmods tid m past future γ : iProp Σ :=
+  per_key_inv_def γ key tmods tid m past ∗ cmt_inv_def γ tmods future.
 
-Lemma tuple_read_safe tid key tmods m past future tuple val found γ :
+Lemma tuple_read_safe tid ts key tmods m past future tuple val found γ :
   head_read future tid key ->
-  ([∗ set] k ∈ keys_all, per_key_inv_def γ k tmods m past) -∗
+  ([∗ set] k ∈ keys_all, per_key_inv_def γ k tmods ts m past) -∗
   cmt_inv_def γ tmods future -∗
   tuple_read tuple tid key val found γ ==∗
-  ([∗ set] k ∈ keys_all, per_key_inv_def γ k tmods m (past ++ [EvRead tid key])) ∗
+  ([∗ set] k ∈ keys_all, per_key_inv_def γ k tmods ts m (past ++ [EvRead tid key])) ∗
   cmt_inv_def γ tmods future ∗
   own_tuple tuple key γ ∗
-  view_ptsto γ key (to_dbval found val) tid.
+  ptuple_ptsto γ key (to_dbval found val) (int.nat tid).
 Admitted.
 
 (*
