src/program_proof/mvcc/vok.sh
@@ -1,0 +1,14 @@
+#!/bin/bash
+
+dir='./src/program_proof/mvcc'
+
+cd ../../../
+files=`find ${dir} -name "${1}*.v" | sed "s/\.v/\.vok/"`
+if [[ -z ${files} ]]; then
+    echo "No target files."
+    exit 1
+fi
+
+echo "Checking:"
+echo "`basename ${files}`"
+make -j4 ${files}
